EvmStructure.thy
@@ -1,0 +1,778 @@
+theory "EvmStructure" 
+
+imports  "lem/Evm" "Hoare"
+  "HoareTripleForInstructions"
+
+begin
+
+(* accessors for variables *)
+type_synonym 'a access = "variable_ctx \<Rightarrow> 'a"
+
+definition const :: "nat \<Rightarrow> nat access" where
+"const w ctx = w"
+
+definition cell :: "nat \<Rightarrow> nat access" where
+"cell w ctx = unat (vctx_storage ctx (word256FromNat w))"
+
+definition arr :: "nat \<Rightarrow> nat \<Rightarrow> (nat \<Rightarrow> nat) access" where
+"arr addr len ctx x = (if x < len then cell (addr+x) ctx else 0)"
+
+definition cannot_modify :: "w256 \<Rightarrow> 'a access \<Rightarrow> bool" where
+"cannot_modify w x = (\<forall>ctx t. x ctx = x (vctx_update_storage w t ctx))" 
+
+lemma cannot_update_const : "cannot_modify addr (const c)"
+apply(simp add:cannot_modify_def const_def)
+done
+
+lemma cannot_update_cell :
+  "addr1 \<noteq> addr2 \<Longrightarrow> cannot_modify addr1 (cell (unat addr2))"
+apply(simp add:cannot_modify_def cell_def word256FromNat_def unat_def
+  vctx_update_storage_def)
+done
+
+lemma s : "(\<forall>x. f x = g x) \<Longrightarrow> f = g"
+apply(auto)
+done
+
+lemma test : "(a::int) mod 100 \<ge> 0"
+apply arith
+done
+
+lemma word_of_int_le :
+ "(word_of_int x :: 256 word) \<le> (word_of_int y :: 256 word) \<Longrightarrow>
+  x mod 2^256 \<le> y mod 2^256" 
+apply (auto simp:uint_word_of_int word_le_def)
+done
+
+lemma l : "(x::int) mod 2^256 < addr \<Longrightarrow> x < 2^256 \<Longrightarrow> x \<ge> 0 \<Longrightarrow>
+  x < addr"
+using int_mod_ge by fastforce
+
+lemma ll : "(word_of_int x :: 256 word) < (addr::256 word) \<Longrightarrow>
+   uint (word_of_int x :: 256 word) < uint addr"
+  by (simp add: word_less_def)
+
+lemma ll_a : "(word_of_int x :: 256 word) \<le> (addr::256 word) \<Longrightarrow>
+   uint (word_of_int x :: 256 word) \<le> uint addr"
+  by (simp add: word_le_def)
+
+lemma ll_b : "(word_of_int x :: 256 word) \<ge> (addr::256 word) \<Longrightarrow>
+   uint (word_of_int x :: 256 word) \<ge> uint addr"
+  by (simp add: word_le_def)
+
+lemma l2 : 
+  assumes a:"(word_of_int x :: 256 word) < (addr::256 word)"
+  and small:"x < 2^256" and  natural:"x \<ge> 0"
+  shows "x < uint addr"
+proof -
+from a and ll have b: "uint (word_of_int x :: 256 word) < uint addr" by auto
+have "uint (word_of_int x :: 256 word) = x mod 2^256" by
+   (auto simp:uint_word_of_int)
+then have "uint (word_of_int x :: 256 word) = x" using natural and small
+  by (simp add: natural int_mod_eq) 
+then show ?thesis using b by auto
+qed
+
+lemma l2_a : 
+  assumes a:"(word_of_int x :: 256 word) \<le> (addr::256 word)"
+  and small:"x < 2^256" and  natural:"x \<ge> 0"
+  shows "x \<le> uint addr"
+proof -
+from a and ll_a have b: "uint (word_of_int x :: 256 word) \<le> uint addr" by auto
+have "uint (word_of_int x :: 256 word) = x mod 2^256" by
+   (auto simp:uint_word_of_int)
+then have "uint (word_of_int x :: 256 word) = x" using natural and small
+  by (simp add: natural int_mod_eq) 
+then show ?thesis using b by auto
+qed
+
+lemma l2_b : 
+  assumes a:"(word_of_int x :: 256 word) \<ge> (addr::256 word)"
+  and small:"x < 2^256" and  natural:"x \<ge> 0"
+  shows "x \<ge> uint addr"
+proof -
+from a and ll_b have b: "uint (word_of_int x :: 256 word) \<ge> uint addr" by auto
+have "uint (word_of_int x :: 256 word) = x mod 2^256" by
+   (auto simp:uint_word_of_int)
+then have "uint (word_of_int x :: 256 word) = x" using natural and small
+  by (simp add: natural int_mod_eq) 
+then show ?thesis using b by auto
+qed
+
+lemma k : 
+  "word_of_int (uint (addr2::256 word) + int x) < addr2 \<Longrightarrow>
+   uint addr2 + int x < 2^256 \<Longrightarrow>
+   False"
+using l2 not_add_less2 of_nat_0_le_iff by fastforce
+
+lemma k_d : 
+  "addr2 + x + 1 \<le> word_of_int (uint (addr2::256 word) + uint x) \<Longrightarrow>
+   uint addr2 + uint x + 1 < 2^256 \<Longrightarrow>
+   uint (addr2 + x + 1) \<le> uint (addr2::256 word) + uint x"
+using l2_b
+apply fastforce
+done
+
+lemma word_size : "uint (w::256 word) < 2^256"
+using word.uint [of w] by simp
+
+lemma k_a : 
+  assumes a: "addr2 + len \<le> (word_of_int (uint addr2 + int x) :: 256 word)"
+  and small:"uint (addr2::256 word) + uint (len::256 word) < 2^256"
+  and xlen: "x < nat (uint len)"
+  shows "False"
+proof -
+  have s1:"uint (addr2 + len :: 256 word) < 2^256" by (rule word_size)
+  from xlen and small have s2:"uint addr2 + int x < 2^256" by auto
+  from small and s1 have com: "uint (addr2 + len) = uint addr2 + uint len"
+    by (meson dual_order.order_iff_strict l2_a not_le order_trans uint_add_lem uint_lt zero_le_numeral zero_le_power)
+  from a have "(word_of_int (uint (addr2 + len)) :: 256 word) \<le>
+   (word_of_int (uint addr2 + int x) :: 256 word)" by auto
+  then have "uint (addr2 + len) mod 2^256 \<le>
+             (uint addr2 + int x) mod 2^256"
+    using word_of_int_le by blast 
+  from this and s1 and s2 have "uint (addr2 + len) \<le> uint addr2 + int x"
+    using a add_nonneg_nonneg l2_b of_nat_0_le_iff uint_nonnegative by blast
+  from this and xlen and com show False by auto
+qed
+
+lemma kk :
+   "uint (addr2::256 word) + uint len < 2^256 \<Longrightarrow>
+    x < nat (uint (len::256 word)) \<Longrightarrow>
+    uint addr2 + int x < 2^256"
+  by linarith
+
+lemma cannot_update_array_small :
+  "addr1 < addr2 \<Longrightarrow>
+   uint (addr2::256 word) + uint (len::256 word) < 2^256 \<Longrightarrow>
+   cannot_modify addr1 (arr (unat addr2) (unat len))"
+apply(simp add:cannot_modify_def cell_def word256FromNat_def unat_def
+  vctx_update_storage_def arr_def)
+apply(auto)
+apply(rule s)
+apply(simp add:cannot_modify_def cell_def word256FromNat_def unat_def
+  vctx_update_storage_def arr_def)
+apply(auto)
+using k kk
+apply fastforce
+done
+
+lemma cannot_update_array_large :
+  "addr1 \<ge> addr2 + len \<Longrightarrow>
+   uint (addr2::256 word) + uint (len::256 word) < 2^256 \<Longrightarrow>
+   cannot_modify addr1 (arr (unat addr2) (unat len))"
+apply(simp add:cannot_modify_def cell_def word256FromNat_def unat_def
+  vctx_update_storage_def arr_def)
+apply(auto)
+apply(rule s)
+apply(simp add:cannot_modify_def cell_def word256FromNat_def unat_def
+  vctx_update_storage_def arr_def)
+apply(auto)
+using k_a
+apply fastforce
+done
+
+(* separation logic statement for cell?
+
+storage :: w256 \<Rightarrow> w256 \<Rightarrow> set_pred
+
+*)
+
+fun storage_array :: "w256 \<Rightarrow> w256 list \<Rightarrow> set_pred" where
+"storage_array ind [] = emp"
+| "storage_array ind (a#b) = storage ind a ** storage_array (ind+1) b"
+
+definition hash :: "w256 \<Rightarrow> w256 \<Rightarrow> w256 option" where
+"hash a b = None"
+
+definition hash3 :: "w256 \<Rightarrow> w256 \<Rightarrow> w256" where
+"hash3 a b = (case hash a b of
+   None \<Rightarrow> undefined
+ | Some h \<Rightarrow> h )"
+
+axiomatization hash2 :: "w256 \<Rightarrow> w256 \<Rightarrow> w256" where
+hash_inj : "hash2 b v1 = hash2 c v2 \<Longrightarrow> b = c"
+and hash_inj2 : "hash2 b v1 = hash2 c v2 \<Longrightarrow> v1 = v2"
+and hash_foo : "hash3 a b = hash2 a b"
+(*
+lemma "False"
+using hash3_def hash_def hash_inj hash_inj2 hash_foo
+*)
+
+fun assoc :: "(w256*w256) list \<Rightarrow> set_pred" where
+  "assoc [] = emp"
+| "assoc ((key,a)#xs) = storage key a ** assoc xs"
+
+(*
+fun mapping :: "w256 \<Rightarrow> (w256*w256) list \<Rightarrow> set_pred" where
+  "mapping ind [] = emp"
+| "mapping ind ((key,a)#tll) = (case super_hash key a of
+    None \<Rightarrow> mapping ind tll (* what is the correct way to handle? *)
+  | Some h \<Rightarrow> storage h a ** mapping ind tll)"
+*)
+
+definition mapping :: "w256 \<Rightarrow> (w256*w256) list \<Rightarrow> set_pred" where
+"mapping ind lst = assoc (map (\<lambda>p. (hash2 ind (fst p), snd p)) lst)"
+
+fun get :: "w256 \<Rightarrow> (w256*w256) list \<Rightarrow> w256" where
+  "get k [] = 0"
+| "get k ((ok,ov)#xs) = (if k = ok then ov else get k xs)"
+
+fun mem :: "w256 \<Rightarrow> (w256*w256) list \<Rightarrow> bool" where
+  "mem k [] = False"
+| "mem k ((ok,ov)#xs) = (k = ok \<or> mem k xs)"
+
+fun remove :: "w256 \<Rightarrow> (w256*w256) list \<Rightarrow> (w256*w256) list" where
+  "remove k [] = []"
+| "remove k ((ok,ov)#xs) =
+   (if k = ok then xs else (ok,ov)#remove k xs)"
+
+(*
+fun add :: "w256 \<Rightarrow> w256 \<Rightarrow> (w256*w256) list \<Rightarrow> (w256*w256) list" where
+  "add k v [] = [(k,v)]"
+| "add k v ((ok,ov)#xs) =
+   (if k = ok then (k,v)#xs else (ok,ov)#add k v xs)"
+*)
+
+fun add :: "w256 \<Rightarrow> w256 \<Rightarrow> (w256*w256) list \<Rightarrow> (w256*w256) list" where
+"add k v lst = (k,v)#remove k lst"
+
+lemma add_not_mem : "\<not> (mem k lst) \<Longrightarrow> add k v lst = (k,v)#lst"
+apply (induction lst)
+apply(auto)
+done
+
+lemma stored :
+   "mem k mp \<Longrightarrow>
+    assoc mp = assoc (remove k mp) ** storage k (get k mp)"
+apply (induction mp)
+apply(auto)
+done
+
+lemma stored_hash_from_mapping :
+   "mem k mp \<Longrightarrow>
+    mapping ind mp =
+    mapping ind (remove k mp) ** storage (hash2 ind k) (get k mp)"
+apply (induction mp)
+apply(auto simp:mapping_def)
+done
+
+lemma minus_test : "a - {x} - {y} = a - {y} - {x}"
+apply auto
+done
+
+lemma mapping_cons :
+   "mapping ind ((k,v)#mp) = storage (hash2 ind k) v ** mapping ind mp"
+apply (induction mp)
+apply(auto simp:mapping_def minus_test)
+done
+
+lemma set_storage1 :
+  assumes a:"mem key m"
+  shows "triple {OutOfGas}
+    (\<langle> h \<le> 1024 \<rangle> **
+     stack (h+1) (hash2 table key) **
+     stack h v **
+     stack_height (h+2) **
+     mapping table m **
+     program_counter k **
+     gas_pred g **
+     continuing)
+    {(k, Storage SSTORE)}
+    (mapping table (add key v m) **
+     program_counter (k+1) **
+     gas_pred (g - Csstore (get key m) v) **
+     stack_height h **
+     continuing)" (is "triple _ ?pre _ ?post")
+proof -
+  from a have good_pre: "?pre =
+     (\<langle> h \<le> 1024 \<rangle> **
+     stack_height (h+2) **
+     stack (h+1) (hash2 table key) **
+     stack h v **
+     program_counter k **
+     storage (hash2 table key) (get key m) **
+     gas_pred g **
+     continuing) **
+     mapping table (remove key m)"
+     (is "?pre = ?presmall ** _")
+     by (auto simp:stored_hash_from_mapping)
+  have good_post: "?post = (
+     stack_height h **
+     program_counter (k+1) **
+     storage (hash2 table key) v **
+     gas_pred (g - Csstore (get key m) v) **
+     continuing) **
+     mapping table (remove key m)" (is "_ = ?postsmall ** _")
+
+     by (auto simp:mapping_cons)
+  have "triple {OutOfGas} ?presmall {(k, Storage SSTORE)} ?postsmall"
+    by (rule sstore_gas_triple)
+  then have "triple {OutOfGas} (?presmall ** mapping table (remove key m))
+      {(k, Storage SSTORE)} (?postsmall ** mapping table (remove key m))"
+    by (rule frame)
+  then show ?thesis using good_pre and good_post by simp
+qed
+
+lemma set_storage2 :
+  assumes a:"\<not> (mem key m)"
+  shows "triple {OutOfGas}
+    (\<langle> h \<le> 1024 \<rangle> **
+     stack (h+1) (hash2 table key) **
+     stack h v **
+     stack_height (h+2) **
+     mapping table m **
+     storage (hash2 table key) 0 **
+     program_counter k **
+     gas_pred g **
+     continuing)
+    {(k, Storage SSTORE)}
+    (mapping table (add key v m) **
+     program_counter (k+1) **
+     gas_pred (g - Csstore 0 v) **
+     stack_height h **
+     continuing)" (is "triple _ ?pre _ ?post")
+proof -
+  have good_pre: "?pre =
+     (\<langle> h \<le> 1024 \<rangle> **
+     stack_height (h+2) **
+     stack (h+1) (hash2 table key) **
+     stack h v **
+     program_counter k **
+     storage (hash2 table key) 0 **
+     gas_pred g **
+     continuing) **
+     mapping table m"
+     (is "?pre = ?presmall ** _")
+     by (auto simp:stored_hash_from_mapping)
+  from a have good_post: "?post = (
+     stack_height h **
+     program_counter (k+1) **
+     storage (hash2 table key) v **
+     gas_pred (g - Csstore 0 v) **
+     continuing) **
+     mapping table m" (is "_ = ?postsmall ** _")
+     by (subst add_not_mem) (auto simp:mapping_cons)
+  have "triple {OutOfGas} ?presmall {(k, Storage SSTORE)} ?postsmall"
+    by (rule sstore_gas_triple)
+  then have "triple {OutOfGas} (?presmall ** mapping table m)
+      {(k, Storage SSTORE)} (?postsmall ** mapping table m)"
+    by (rule frame)
+  then show ?thesis using good_pre and good_post by simp
+qed
+
+definition perhaps_alloc ::
+   "w256 \<Rightarrow> w256 \<Rightarrow> (w256*w256) list \<Rightarrow> set_pred" where
+"perhaps_alloc ind k lst =
+    (if mem k lst then emp else storage (hash2 ind k) 0)"
+
+lemma mem_perhaps :
+  "mem key m \<Longrightarrow>
+   mapping table m ** perhaps_alloc table key m =
+   mapping table m"
+apply(auto simp:perhaps_alloc_def)
+done
+
+lemma mem_perhaps_not :
+  "\<not>mem key m \<Longrightarrow>
+   mapping table m ** perhaps_alloc table key m =
+   mapping table m ** storage (hash2 table key) 0"
+apply(auto simp:perhaps_alloc_def)
+done
+
+lemma not_mem_get_zero : "\<not>mem key m \<Longrightarrow> get key m = 0"
+apply (induction m)
+apply (auto)
+done
+
+lemma set_storage :
+  "triple {OutOfGas}
+    (\<langle> h \<le> 1024 \<rangle> **
+     stack (h+1) (hash2 table key) **
+     stack h v **
+     stack_height (h+2) **
+     (mapping table m ** perhaps_alloc table key m) **
+     program_counter k **
+     gas_pred g **
+     continuing)
+    {(k, Storage SSTORE)}
+    (mapping table (add key v m) **
+     program_counter (k+1) **
+     gas_pred (g - Csstore (get key m) v) **
+     stack_height h **
+     continuing)"
+apply (cases "mem key m")
+apply(subst mem_perhaps)
+apply(simp)
+using set_storage1
+apply(simp)
+apply(subst mem_perhaps_not)
+apply(simp)
+apply(subst not_mem_get_zero)
+apply(simp)
+using set_storage2
+apply(auto)
+done
+
+lemma get_storage1 :
+  assumes a:"mem key m"
+  shows
+  "triple {OutOfGas}
+    (\<langle>h \<le> 1023 \<and> unat bn \<ge> 2463000 \<rangle> **
+     stack_height (h+1) **
+     stack h (hash2 table key) **
+     mapping table m **
+     block_number_pred bn **
+     program_counter k **
+     gas_pred g **
+     continuing)
+    {(k, Storage SLOAD)}
+    (stack h (get key m) **
+     mapping table m **
+     program_counter (k+1) **
+     block_number_pred bn **
+     gas_pred (g - Gsload (unat bn)) **
+     stack_height (h+1) **
+     continuing)"
+ (is "triple _ ?pre _ ?post")
+proof -
+  from a have good_pre: "?pre =
+     (\<langle>h \<le> 1023 \<and> unat bn \<ge> 2463000 \<rangle> **
+     block_number_pred bn ** stack_height (h + 1) **
+     stack h (hash2 table key) **
+     program_counter k **
+     storage (hash2 table key) (get key m) **
+     gas_pred g ** continuing) **
+     mapping table (remove key m)"
+     (is "?pre = ?presmall ** _")
+     by (auto simp:stored_hash_from_mapping)
+  have good_post: "?post = (
+     block_number_pred bn ** stack_height (h + 1) **
+     stack h (get key m) ** 
+     program_counter (k + 1) **
+     storage (hash2 table key) (get key m) **
+     gas_pred (g - Gsload (unat bn)) ** continuing ) **
+     mapping table (remove key m)" (is "_ = ?postsmall ** _")
+     by (subst stored_hash_from_mapping) (auto simp:a)
+  have "triple {OutOfGas} ?presmall {(k, Storage SLOAD)} ?postsmall"
+    by (rule sload_gas_triple)
+  then have "triple {OutOfGas} (?presmall ** mapping table (remove key m))
+      {(k, Storage SLOAD)} (?postsmall ** mapping table (remove key m))"
+    by (rule frame)
+  then show ?thesis using good_pre and good_post by simp
+qed
+
+lemma get_storage2 :
+  assumes a:"\<not>mem key m"
+  shows
+  "triple {OutOfGas}
+    (\<langle>h \<le> 1023 \<and> unat bn \<ge> 2463000 \<rangle> **
+     stack_height (h+1) **
+     stack h (hash2 table key) **
+     mapping table m **
+     storage (hash2 table key) (get key m) **
+     block_number_pred bn **
+     program_counter k **
+     gas_pred g **
+     continuing)
+    {(k, Storage SLOAD)}
+    (stack h (get key m) **
+     mapping table m **
+     storage (hash2 table key) (get key m) **
+     program_counter (k+1) **
+     block_number_pred bn **
+     gas_pred (g - Gsload (unat bn)) **
+     stack_height (h+1) **
+     continuing)"
+ (is "triple _ ?pre _ ?post")
+proof -
+  from a have good_pre: "?pre =
+     (\<langle>h \<le> 1023 \<and> unat bn \<ge> 2463000 \<rangle> **
+     block_number_pred bn ** stack_height (h + 1) **
+     stack h (hash2 table key) **
+     program_counter k **
+     storage (hash2 table key) 0 **
+     gas_pred g ** continuing) **
+     mapping table m"
+     (is "?pre = ?presmall ** _")
+     by (simp add:not_mem_get_zero)
+  from a have good_post: "?post = (
+     block_number_pred bn ** stack_height (h + 1) **
+     stack h 0 ** 
+     program_counter (k + 1) **
+     storage (hash2 table key) 0 **
+     gas_pred (g - Gsload (unat bn)) ** continuing ) **
+     mapping table m" (is "_ = ?postsmall ** _")
+     by (simp add:not_mem_get_zero)
+  have "triple {OutOfGas} ?presmall {(k, Storage SLOAD)} ?postsmall"
+    by (rule sload_gas_triple)
+  then have "triple {OutOfGas} (?presmall ** mapping table m)
+      {(k, Storage SLOAD)} (?postsmall ** mapping table m)"
+    by (rule frame)
+  then show ?thesis using good_pre and good_post by simp
+qed
+
+lemma get_storage :
+  "triple {OutOfGas}
+    (\<langle>h \<le> 1023 \<and> unat bn \<ge> 2463000 \<rangle> **
+     stack_height (h+1) **
+     stack h (hash2 table key) **
+     ( mapping table m ** perhaps_alloc table key m ) **
+     block_number_pred bn **
+     program_counter k **
+     gas_pred g **
+     continuing)
+    {(k, Storage SLOAD)}
+    (stack h (get key m) **
+     ( mapping table m ** perhaps_alloc table key m ) **
+     program_counter (k+1) **
+     block_number_pred bn **
+     gas_pred (g - Gsload (unat bn)) **
+     stack_height (h+1) **
+     continuing)"
+apply (cases "mem key m")
+apply(subst mem_perhaps)
+apply(simp)
+apply(subst mem_perhaps)
+apply(simp)
+using get_storage1
+apply(simp)
+apply(subst mem_perhaps_not)
+apply(simp)
+apply(subst mem_perhaps_not)
+apply(simp)
+using get_storage2
+apply(auto simp:not_mem_get_zero)
+done
+
+definition zero_table :: "w256 \<Rightarrow> state_element set" where
+"zero_table table = {StorageElm (hash2 table key,0) | key. True}"
+
+(* set with exactly correct elems *)
+definition alloc_zero_table :: "w256 \<Rightarrow> set_pred" where
+"alloc_zero_table table = (\<lambda>st. st = zero_table table)"
+
+definition alloc_zero_tables :: "w256 \<Rightarrow> w256 \<Rightarrow> set_pred" where
+"alloc_zero_tables t1 t2 = (\<lambda>st. st = zero_table t1 \<union> zero_table t2)"
+
+definition memory :: "w256 \<Rightarrow> w256 \<Rightarrow> set_pred" where
+"memory ind w = memory_range ind (word_rsplit w)"
+
+(*
+lemma hash_inj : "hash2 a b = hash2 a c \<Longrightarrow>
+   b = c \<or> hash2 a b = undefined \<or> hash2 a c = undefined"
+apply(simp add:hash2_def hash_def)
+done
+
+lemma hash_inj2 : "hash2 b v1 = hash2 c v2 \<Longrightarrow>
+   b = c \<or> hash2 b v1 = undefined \<or> hash2 c v2 = undefined"
+apply(simp add:hash2_def hash_def)
+done
+
+lemma undef : "hash2 undefined undefined = undefined"
+apply(simp add:hash2_def hash_def)
+done
+
+lemma foo : "(1::int) \<noteq> undefined"
+apply auto
+*)
+
+lemma separate_table :
+  "a \<noteq> b \<Longrightarrow> zero_table a \<inter> zero_table b = {}"
+apply (auto simp:zero_table_def hash_inj)
+done
+
+lemma separate_table2 :
+  "a \<noteq> b \<Longrightarrow>
+  alloc_zero_tables a b = alloc_zero_table a ** alloc_zero_table b"
+apply(auto simp:alloc_zero_table_def alloc_zero_tables_def
+   sep_def separate_table)
+done
+
+definition assoc_set ::
+  "(w256*w256) list \<Rightarrow> state_element set" where
+"assoc_set m = {StorageElm (a,b) | a b. (a,b) \<in> set m}"
+
+definition mapping_set ::
+  "w256 \<Rightarrow> (w256*w256) list \<Rightarrow> state_element set" where
+"mapping_set table m =
+   assoc_set (map (\<lambda>p. (hash2 table (fst p), snd p)) m)"
+(*
+   {StorageElm (hash2 table a,b) | a b. (a,b) \<in> set m}"
+*)
+
+definition mapping_zero ::
+   "w256 \<Rightarrow> (w256*w256) list \<Rightarrow> state_element set" where
+"mapping_zero table m = zero_table table - mapping_set table m"
+
+definition alloc_zero ::
+   "w256 \<Rightarrow> (w256*w256) list \<Rightarrow> set_pred" where
+"alloc_zero table m = (\<lambda>st. st = mapping_zero table m)"
+
+lemma start_table : "alloc_zero_table t = alloc_zero t [] **
+                     mapping t []"
+apply(auto simp:alloc_zero_table_def alloc_zero_def sep_def
+  mapping_def mapping_zero_def mapping_set_def emp_def
+  assoc_set_def)
+done
+
+(* does not work because may have several times
+  the same element*)
+definition diff_keys :: "(w256*w256) list \<Rightarrow> bool" where
+"diff_keys m = (card (set (map fst m)) = length m)"
+
+lemma card_insert : "k \<in> s \<Longrightarrow> card (insert k s) = card s"
+apply(auto simp:Set.insert_absorb)
+done
+
+lemma insert_union : "k \<notin> s \<Longrightarrow> insert k s = s \<union> {k}"
+apply(auto)
+done
+
+lemma card_insert_cmp : "card (insert k s) \<ge> card s"
+apply (cases "k \<notin> s")
+apply(auto simp:Set.insert_absorb)
+apply (metis card_infinite card_insert_le card_mono eq_iff subset_insertI)
+done
+
+lemma card_insert_alt :
+  "finite s \<Longrightarrow>
+   card (insert k s) = card s + 1 \<or> card (insert k s) = card s"
+apply (cases "k \<notin> s")
+apply(auto simp:Set.insert_absorb)
+done
+
+lemma card_insert_alt2 :
+  "finite s \<Longrightarrow>
+   k \<notin> s \<Longrightarrow>
+   card (insert k s) = card s + 1"
+apply(auto)
+done
+
+lemma card_insert_len :
+ "card (insert k (set l)) = length l + 1 \<Longrightarrow>
+  card (set l) = length l"
+apply (cases "k \<notin> set l")
+apply(simp)
+apply(auto)
+apply(simp add:Set.insert_absorb)
+using card_length [of l]
+apply arith
+done
+
+lemma helper : "length l = length (map fst l)"
+apply auto
+done
+
+lemma diff_keys_cons : "diff_keys ((k,v)#l) \<Longrightarrow> diff_keys l"
+apply (subst diff_keys_def)
+apply (subst (asm) diff_keys_def)
+apply (subst helper)
+apply (rule card_insert_len)
+apply(auto)
+done
+
+lemma card_set_cons :
+    "p \<in> set m \<Longrightarrow>
+    card (set (p # m)) = length (p # m) \<Longrightarrow>
+    False"
+apply(simp add:Set.insert_absorb)
+using card_length [of m]
+apply arith
+done
+
+lemma easy : "p \<in> set m \<Longrightarrow> f p \<in> set (map f m)"
+apply (induction m)
+apply auto
+done
+
+lemma cannot_add_same :
+  "(a, b) \<in> set m \<Longrightarrow>
+   diff_keys ((a,b)#m) \<Longrightarrow> False"
+apply (subst (asm) diff_keys_def)
+apply (subst (asm) helper)
+apply (rule card_set_cons [of "a" "map fst m"])
+using easy [of "(a,b)" m fst]
+apply auto
+done
+
+lemma assoc_as_set :
+   "diff_keys m \<Longrightarrow> assoc m s = (s = assoc_set m)"
+apply (induction m arbitrary:s)
+apply(simp add:assoc_set_def emp_def)
+subgoal for a m s
+apply (induction a)
+apply(simp)
+subgoal for aa bb
+using diff_keys_cons [of aa bb m]
+apply(simp)
+apply (rule pqqp)
+apply(simp add:assoc_set_def emp_def)
+apply blast
+apply(simp add:assoc_set_def emp_def)
+apply auto
+using cannot_add_same
+apply fastforce
+done
+
+lemma mapping_as_set :
+  "diff_keys m \<Longrightarrow> 
+   mapping t m s = (s = mapping_set t m)"
+apply(simp add:mapping_def mapping_set_def emp_def)
+using assoc_as_set
+
+apply(simp add:mapping_set_def)
+
+lemma alloc_table :
+   "alloc_zero t m ** mapping t m =
+    alloc_zero t (p#m) ** mapping t (p#m)"
+apply(auto simp:alloc_zero_table_def alloc_zero_def sep_def
+  emp_def
+  zero_table_def)
+apply(rule s)
+apply(auto)
+
+(*
+lemma set_storage :
+  "triple {OutOfGas}
+    (memory 0 table ** memory 1 key ** stack h v **
+     stack_height (h+1) **
+     mapping table m **
+     program_counter k **
+     gas_pred g **
+     continuing)
+    {(k,Stack (PUSH_N (word_rsplit 64))),
+     (k+1,Stack (PUSH_N (word_rsplit 0))),
+     (k+2, Arith SHA3),
+     (k+3, Storage SSTORE)}
+    (memory 0 table ** memory 1 key ** stack h v **
+     mapping table (add key v m) **
+     program_counter (k+4) **
+     gas_pred g **
+     stack_height h **
+     continuing)"
+
+lemma get_storage :
+  "triple {OutOfGas}
+    (memory 0 table ** memory 1 key **
+     stack_height h **
+     mapping table m **
+     program_counter k **
+     gas_pred g **
+     continuing)
+    {(k,Stack (PUSH_N (word_rsplit 64))),
+     (k+1,Stack (PUSH_N (word_rsplit 0))),
+     (k+2, Arith SHA3),
+     (k+3, Storage SLOAD)}
+    (memory 0 table ** memory 1 key ** stack h v **
+     mapping table m **
+     program_counter (k+4) **
+     gas_pred g **
+     stack (h+1) **
+     stack_height (h+1) **
+     continuing)"
+*)
+
+end
+
+
